theories/Decidability/UntypedTermination.v
@@ -1,0 +1,610 @@
+(** * LogRel.Decidability.UntypedTermination: the implementation always terminates on well-typed inputs. *)
+From Coq Require Import Nat Lia Arith.
+From Equations Require Import Equations.
+From LogRel.AutoSubst Require Import core unscoped Ast Extra.
+From LogRel Require Import BasicAst Context Notations UntypedReduction Weakening DeclarativeTyping DeclarativeInstance GenericTyping NormalForms.
+From LogRel Require Import Validity LogicalRelation Fundamental DeclarativeSubst TypeConstructorsInj AlgorithmicTyping BundledAlgorithmicTyping Normalisation AlgorithmicConvProperties AlgorithmicTypingProperties.
+From LogRel Require Import UntypedAlgorithmicConversion.
+From LogRel Require Import Utils. (* at the end, to get the right easy tactic… *)
+From LogRel.Decidability Require Import Functions UntypedFunctions Soundness UntypedSoundness Completeness UntypedCompleteness.
+From PartialFun Require Import Monad PartialFun MonadExn.
+
+Import DeclarativeTypingProperties AlgorithmicTypingData.
+
+Set Universe Polymorphism.
+
+
+Lemma uconv_sound_decl :
+  UAlgoConvInductionConcl
+    (fun t u => 
+      (forall Γ, [Γ |-[de] t] × [Γ |-[de] u] -> [Γ |-[de] t ≅ u]) ×
+      (forall Γ A, [Γ |-[de] t : A] × [Γ |-[de] u : A] -> [Γ |-[de] t ≅ u : A]))
+
+    (fun t u =>
+      (forall Γ, [Γ |-[de] t] × [Γ |-[de] u] -> [Γ |-[de] t ≅ u]) ×
+      (forall Γ A, isType A -> [Γ |-[de] t : A] × [Γ |-[de] u : A] -> [Γ |-[de] t ≅ u : A]))
+
+    (fun t u =>
+      forall Γ, well_typed Γ t × well_typed Γ u ->
+      ∑ A'', [Γ |-[de] t ≅ u : A'']).
+Proof.
+  split ; [..|split].
+  all: intros t u Hconv.
+  1-2: split.
+  - intros * [].
+    eapply uconv_sound in Hconv as [?%algo_conv_sound _]; eauto.
+  - intros * [].
+    eapply uconv_sound in Hconv as [_ ?%algo_conv_sound]; eauto.
+  - intros * [].
+    eapply uconv_sound in Hconv as [?%algo_conv_sound _]; eauto. 
+  - intros * ? [].
+    eapply uconv_sound in Hconv as [_ ?%algo_conv_sound]; eauto.
+  - intros * [].
+    eapply uconv_sound in Hconv as [? []%algo_conv_sound] ; eauto.
+Qed.
+
+
+#[universes(polymorphic)]Definition uconv_str_type
+    (x : uconv_state × term × term)
+    (r : exn errors unit) : Type :=
+  match x,r with
+  | (s,t,u), success _ =>
+      forall (Γ Δ : context) (ρ : Δ ≤ Γ) t' u',
+      t = t'⟨ρ⟩ -> u = u'⟨ρ⟩ -> graph _uconv (s,t',u') ok
+  | (s,t,u), exception e => 
+    forall (Γ Δ : context) (ρ : Δ ≤ Γ) t' u',
+    t = t'⟨ρ⟩ -> u = u'⟨ρ⟩ -> ∑ e', graph _uconv (s,t',u') (exception e')
+  end.
+
+Lemma wh_red_str (Γ Δ : context) (ρ : Δ ≤ Γ) t v :
+  graph wh_red t⟨ρ⟩ v ->
+  ∑ v', v = v'⟨ρ⟩ × graph wh_red t v'.
+Proof.
+Admitted.
+
+Lemma _uconv_str :
+  funrect _uconv (fun _ => True) uconv_str_type.
+Proof.
+Admitted.
+
+Lemma uconv_expand_ne_eta n n' :
+  whne n ->
+  whne n' ->
+  domain _uconv (tm_state, eta_expand n, eta_expand n') ->
+  domain _uconv (ne_state, n, n').
+Proof.
+  intros w w' [v g].
+  unfold graph in g.
+  simp _uconv uconv_tm in g ; cbn in g.
+  apply (orec_graph_call_inv _uconv) in g as [? [red g]] ; cbn in *.
+  eapply red_sound in red as [<-%red_whne _].
+  2: now constructor ; apply whne_ren.
+  apply (orec_graph_call_inv _uconv) in g as [? [red g]] ; cbn in *.
+  eapply red_sound in red as [<-%red_whne _].
+  2: now constructor ; apply whne_ren.
+  apply (orec_graph_rec_inv _uconv) in g as [? [g _]] ; cbn in *.
+  simp _uconv uconv_tm_red in g.
+  apply (orec_graph_rec_inv _uconv) in g as [? [g _]] ; cbn in *.
+  simp _uconv uconv_ne to_neutral_diag in g ; cbn in *.
+  apply (orec_graph_rec_inv _uconv) in g as [r [g _]] ; cbn in *.
+  unshelve eapply funrect_graph in g.
+  4: apply _uconv_str.
+  2: now cbn.
+  cbn in g.
+  destruct r.
+  - eexists.
+    eapply g.
+    all: unshelve erewrite <- wk1_ren_on ; try reflexivity.
+    1: exact ε.
+    exact (tRel 0).
+  - edestruct g ; cycle -1.
+    now eexists.
+    all: unshelve erewrite <- wk1_ren_on ; try reflexivity.
+    1: exact ε.
+    exact (tRel 0).
+Qed.
+
+Lemma uconv_expand_ne_fst n n' :
+    whne n ->
+    whne n' ->
+    domain _uconv (tm_state, tFst n, tFst n') ->
+    domain _uconv (ne_state, n, n').
+  Proof.
+    intros w w' [v g].
+    unfold graph in g.
+    simp _uconv uconv_tm in g ; cbn in g.
+    apply (orec_graph_call_inv _uconv) in g as [? [red g]] ; cbn in *.
+    eapply red_sound in red as [<-%red_whne _].
+    2: now constructor.
+    apply (orec_graph_call_inv _uconv) in g as [? [red g]] ; cbn in *.
+    eapply red_sound in red as [<-%red_whne _].
+    2: now constructor.
+    apply (orec_graph_rec_inv _uconv) in g as [? [g _]] ; cbn in *.
+    simp _uconv uconv_tm_red in g.
+    apply (orec_graph_rec_inv _uconv) in g as [? [g _]] ; cbn in *.
+    simp _uconv uconv_ne to_neutral_diag in g ; cbn in *.
+    apply (orec_graph_rec_inv _uconv) in g as [r [g _]] ; cbn in *.
+    now eexists.
+Qed.
+
+Lemma uconv_expand Γ A t t' B u u':
+    [Γ |- t : A] ->
+    [t ⤳* t'] ->
+    [Γ |- u : B] ->
+    [u ⤳* u'] ->
+    domain _uconv (tm_state, t, u) ->
+    domain _uconv (tm_state, t', u').
+  Proof.
+    intros ? [red ?]%dup ? [red' ?]%dup [v g] ; refold.
+    unfold graph in g.
+    simp _uconv uconv_tm in g ; cbn in g.
+    apply (orec_graph_call_inv _uconv) in g as [? [[? w]%red_sound g]] ; cbn in *.
+    apply (orec_graph_call_inv _uconv) in g as [? [[? w']%red_sound g]] ; cbn in *.
+    apply (orec_graph_rec_inv _uconv) in g as [? [g _]] ; cbn in *.
+    eapply whred_red_det in red, red' ; cycle -1 ; tea.
+    apply compute_domain.
+    simp _uconv uconv_tm ; cbn.
+    split.
+    1:{
+      eexists ; cbn.
+      eapply wh_red_complete_whnf_tm ; tea.
+      now eapply subject_reduction_raw.
+    }
+    intros ? [ ]%red_sound.
+    eapply whred_det in red ; tea ; subst.
+    split.
+    1:{
+      eexists ; cbn.
+      eapply wh_red_complete_whnf_tm ; tea.
+      now eapply subject_reduction_raw.
+    }
+    intros ? [ ]%red_sound.
+    eapply whred_det in red' ; tea ; subst.
+    split.
+    2: easy.
+    now eexists.
+Qed.
+
+Import DeclarativeTypingProperties.
+
+Section ConversionTerminates.
+
+
+Let PTyEq (Γ : context) (A B : term) :=
+  forall B',
+  [Γ |-[de] A] × [Γ |-[de] B'] ->
+  domain _uconv (tm_state,A,B').
+Let PTyRedEq (Γ : context) (A B : term) :=
+  forall B',
+  isType B' ->
+  [Γ |-[de] A] × [Γ |-[de] B'] ->
+  domain _uconv (tm_red_state,A,B').
+Let PNeEq (Γ : context) (A t u : term) :=
+  forall u',
+  whne u' ->
+  well_typed (ta := de) Γ t × well_typed (ta := de) Γ u' ->
+  domain _uconv (ne_state,t,u').
+Let PTmEq (Γ : context) (A t u : term) :=
+  forall u',
+  [Γ |-[de] t : A] × [Γ |-[de] u' : A] ->
+  domain _uconv (tm_state,t,u').
+Let PTmRedEq (Γ : context) (A t u : term) :=
+  forall u',
+  whnf u' ->
+  [Γ |-[de] t : A] × [Γ |-[de] u' : A] ->
+  domain _uconv (tm_red_state,t,u').
+
+Ltac split_tm :=
+  split ;
+  [ intros * ? [Hz%type_isType Hz'%type_isType] ;
+    [solve [inversion Hz ; inv_whne | inversion Hz' ; inv_whne] | ..] ; solve [ now constructor | now apply isType_whnf]
+  |..].
+
+Theorem _uconv_terminates :
+  AlgoConvInductionConcl PTyEq PTyRedEq PNeEq PNeEq PTmEq PTmRedEq.
+Proof.
+  subst PTyEq PTyRedEq PNeEq PTmEq PTmRedEq.
+  apply AlgoConvInduction.
+
+  - intros * ?? HA IHA * [? Hconcl]%dup.
+    apply compute_domain.
+    simp _conv conv_ty.
+    cbn.
+    split.
+    1: eapply wh_red_complete ; now exists istype.
+    intros A'' []%red_sound.
+    split.
+    1: eapply wh_red_complete ; now exists istype.
+    intros B'' []%red_sound.
+    replace A'' with A'
+      by (eapply whred_det ; tea ; eapply algo_conv_wh in HA as [] ; gen_typing).
+
+    eapply typeConvRed_prem2, IHA in Hconcl as [] ; eauto.
+    2: now eapply type_isType.
+    split ; [now eexists|..].
+    now intros [] ; cbn.
+    
+  - intros * ???? * wB' [Hconcl]%dup.
+    apply compute_domain.
+    simp _uconv uconv_tm_red.
+    destruct wB'.
+    all: simp build_nf_view2 ; cbn ; try easy.
+    2: now unshelve erewrite whne_nf_view1 ; cbn.
+    
+    eapply typePiCongAlg_prem0 in Hconcl as [Hpre0 []]%dup.
+    split ; [eauto | intros [] ; cbn ; [|easy]].
+
+    intros [Hpost0 _]%implem_uconv_graph%uconv_sound_decl ; eauto.
+    eapply typePiCongAlg_prem1 in Hpost0 ; eauto.
+
+  - intros * wB' ?.
+    apply compute_domain.
+    simp _uconv uconv_tm_red.
+    destruct wB'.
+    all: simp build_nf_view2 ; cbn ; try easy.
+    now unshelve erewrite whne_nf_view1 ; cbn.
+
+  - intros * wB' ?.
+    apply compute_domain.
+    simp _uconv uconv_tm_red.
+    destruct wB'.
+    all: simp build_nf_view2 ; cbn ; try easy.
+    now unshelve erewrite whne_nf_view1 ; cbn.
+  
+  - intros * wB' ?.
+    apply compute_domain.
+    simp _uconv uconv_tm_red.
+    destruct wB'.
+    all: simp build_nf_view2 ; cbn ; try easy.
+    now unshelve erewrite whne_nf_view1 ; cbn.
+
+  - intros * ? ? ? ? * wB' [Hconcl]%dup.
+    apply compute_domain.
+    simp _uconv uconv_tm_red.
+    destruct wB'.
+    all: simp build_nf_view2 ; cbn ; try easy.
+    2: now unshelve erewrite whne_nf_view1 ; cbn.
+    
+    eapply typeSigCongAlg_prem0 in Hconcl as [Hpre0 []]%dup.
+    split ; [eauto | intros [] ; cbn ; [|easy]].
+
+    intros [Hpost0 _]%implem_uconv_graph%uconv_sound_decl ; eauto.
+    eapply typeSigCongAlg_prem1 in Hpost0 ; eauto.
+
+  - intros * ? ? ? ? ? ? * wB' [Hconcl]%dup.
+    apply compute_domain.
+    simp _uconv uconv_tm_red.
+    destruct wB'.
+    all: simp build_nf_view2 ; cbn ; try easy.
+    2: now unshelve erewrite whne_nf_view1 ; cbn.
+
+    eapply typeIdCongAlg_prem0 in Hconcl as [Hpre0 []]%dup.
+    split ; [eauto | intros [] ; cbn ; [|easy]].
+
+    intros [[Hpost0]%dup _]%implem_uconv_graph%uconv_sound_decl ; eauto.
+    eapply typeIdCongAlg_prem1 in Hpost0 as [[] Hpre1]%dup ; eauto.
+    split ; [eauto | intros [] ; cbn ; [|easy]].
+
+    intros [_ Hpost1]%implem_uconv_graph%uconv_sound_decl ; eauto.
+    eapply typeIdCongAlg_prem2 in Hpost1 ; eauto.
+    
+  - intros * ?? ?? * wB' [Hconcl]%dup.
+    apply compute_domain.
+    simp _uconv uconv_tm_red build_nf_view2.
+    destruct wB' ; cbn.
+    1-6: now unshelve erewrite whne_nf_view1 ; cbn.
+    do 2 (unshelve erewrite whne_nf_view1 ; tea ; cbn).
+
+    eapply typeNeuConvAlg_prem2 in Hconcl as [Hpre0 []]%dup ; eauto.
+
+  - intros ? n ? ? * wu' [Hconcl]%dup.
+    apply compute_domain.
+    destruct wu' as [n'| | | | | |].
+    all: simp _uconv uconv_ne to_neutral_diag ; cbn ; try easy.
+    now destruct (Nat.eqb_spec n n') ; cbn.
+
+  - intros * Hm ? ?? * wu' [Hconcl]%dup.
+    apply compute_domain.
+    destruct wu'.
+    all: simp _uconv uconv_ne to_neutral_diag ; cbn; try exact I.
+
+    eapply neuAppCongAlg_prem0 in Hconcl as [Hpre0 []]%dup ; eauto.
+    split ; [eauto | intros [] ; cbn ; [|easy]].
+
+    inversion Hm as [????? Hm'] ; refold ; subst.
+    eintros [? Hpost1]%implem_uconv_graph%uconv_sound ; eauto.
+    eapply algo_conv_det in Hm' ; tea ; subst.
+    eapply neuConvRed in Hpost1 ; refold ; tea. 
+    eapply algo_conv_sound, neuAppCongAlg_prem1 in Hpost1 ; eauto.
+
+  - intros * Hn ? ?? ?? ?? * wu' [Hconcl]%dup.
+    apply compute_domain.
+    destruct wu'.
+    all: simp _uconv uconv_ne to_neutral_diag ; cbn; try exact I.
+
+    eapply neuNatElimCong_prem0 in Hconcl as [Hpre0 []]%dup ; eauto.
+    split ; [eauto | intros [] ; cbn ; [|easy]].
+
+    inversion Hn as [????? Hm'] ; refold ; subst.
+    eintros [? Hpost1]%implem_uconv_graph%uconv_sound ; eauto.
+    eapply algo_conv_det in Hm' ; tea ; subst.
+    eapply neuConvRed in Hpost1 ; refold ; tea. 
+    eapply algo_conv_sound in Hpost1 as [[] [Hpost1]%dup]%dup ; eauto.
+    eapply neuNatElimCong_prem1 in Hpost1 as [[]]%dup ; eauto.
+    split ; [eauto | intros [] ; cbn ; [|easy]].
+
+    intros [[Hpost2]%dup _]%implem_uconv_graph%uconv_sound_decl ; eauto.
+    eapply neuNatElimCong_prem2 in Hpost2 as [[]]%dup ; eauto.
+    split ; [eauto | intros [] ; cbn ; [|easy]].
+
+    intros [_ [Hpost3]%dup]%implem_uconv_graph%uconv_sound_decl ; eauto.
+    eapply neuNatElimCong_prem3 in Hpost3 ; eauto.
+
+  - intros * Hn ? ?? * wu' [Hconcl]%dup.
+    apply compute_domain.
+    destruct wu'.
+    all: simp _uconv uconv_ne to_neutral_diag ; cbn; try exact I.
+
+    eapply neuEmptyElimCong_prem0 in Hconcl as [Hpre0 []]%dup ; eauto.
+    split ; [eauto | intros [] ; cbn ; [|easy]].
+
+    inversion Hn as [????? Hm'] ; refold ; subst.
+    eintros [? Hpost1]%implem_uconv_graph%uconv_sound ; eauto.
+    eapply algo_conv_det in Hm' ; tea ; subst.
+    eapply neuConvRed in Hpost1 ; refold ; tea. 
+    eapply algo_conv_sound in Hpost1 as [[] [Hpost1]%dup]%dup ; eauto.
+    eapply neuEmptyElimCong_prem1 in Hpost1 ; eauto.
+
+  - intros * Hn ? * wu' [Hconcl]%dup.
+    apply compute_domain.
+    destruct wu'.
+    all: simp _uconv uconv_ne to_neutral_diag ; cbn; try exact I.
+
+    eapply neuFstCongAlg_prem0 in Hconcl ; eauto.
+    
+  - intros * Hn ? * wu' [Hconcl]%dup.
+    apply compute_domain.
+    destruct wu'.
+    all: simp _uconv uconv_ne to_neutral_diag ; cbn; try exact I.
+
+    eapply neuSndCongAlg_prem0 in Hconcl ; eauto.
+
+  - intros * _ * _ * _ * He ?? ?? ?? * wu' [Hconcl]%dup.
+    apply compute_domain.
+    destruct wu'.
+    all: simp _uconv uconv_ne to_neutral_diag ; cbn; try exact I.
+
+    eapply neuIdElimCong_prem0 in Hconcl as [Hpre0 []]%dup ; eauto.
+    split ; [eauto | intros [] ; cbn ; [|easy]].
+
+    inversion He as [????? He'] ; refold ; subst.
+    eintros [? Hpost1]%implem_uconv_graph%uconv_sound ; eauto.
+    eapply algo_conv_det in He' ; tea ; subst.
+    eapply neuConvRed in Hpost1 ; refold ; tea. 
+    eapply algo_conv_sound in Hpost1 as [[] [Hpost1]%dup]%dup ; eauto.
+    eapply neuIdElimCong_prem1 in Hpost1 as [[]]%dup ; eauto.
+    repeat erewrite <- wk1_ren_on.
+    split ; [eauto | intros [] ; cbn ; [|easy]].
+
+    intros [[Hpost2]%dup _]%implem_uconv_graph%uconv_sound_decl ; eauto.
+    eapply neuIdElimCong_prem2 in Hpost2 ; eauto.
+
+  - eauto.
+
+  - intros * ??? []%algo_conv_wh IH * [Hconcl []]%dup.
+    apply compute_domain.
+    simp _uconv uconv_tm ; cbn.
+
+    split.
+    1: eapply wh_red_complete ; now eexists (isterm _).
+    intros t'' []%red_sound.
+    split.
+    1: eapply wh_red_complete ; now eexists (isterm _).
+    intros u'' []%red_sound.
+
+    replace t'' with t' in * by (eapply whred_det ; eassumption).
+
+    eapply termConvRed_prem3 in Hconcl ; eauto.
+
+  - intros * ?? ?? * wu' [Hconcl []]%dup.
+    apply compute_domain.
+    simp _uconv uconv_tm_red build_nf_view2.
+    eapply Uterm_isType in wu' ; tea.
+    destruct wu' ; cbn ; try exact I.
+    2: now unshelve erewrite whne_nf_view1 ; cbn.
+
+    eapply termPiCongAlg_prem0 in Hconcl as [Hpre0 []]%dup.
+    split ; [eauto | intros [] ; cbn ; [|easy]].
+
+    intros [_ Hpost0]%implem_uconv_graph%uconv_sound_decl ; eauto.
+    eapply termPiCongAlg_prem1 in Hpost0 ; eauto.
+
+  - intros * wu' [Hconcl []]%dup.
+    apply compute_domain.
+    simp _uconv uconv_tm_red build_nf_view2.
+    eapply Uterm_isType in wu' ; tea.
+    destruct wu' ; cbn ; try exact I.
+    now unshelve erewrite whne_nf_view1 ; cbn.
+
+  - intros * wu' [Hconcl []]%dup.
+    apply compute_domain.
+    simp _uconv uconv_tm_red build_nf_view2.
+    eapply nat_isNat in wu' ; tea.
+    destruct wu' ; cbn ; try exact I.
+    now unshelve erewrite whne_nf_view1 ; cbn.
+
+  - intros * ?? * wu' [Hconcl []]%dup.
+    apply compute_domain.
+    simp _uconv uconv_tm_red build_nf_view2.
+    eapply nat_isNat in wu' ; tea.
+    destruct wu' ; cbn ; try exact I.
+    2: now unshelve erewrite whne_nf_view1 ; cbn.
+
+    eapply termSuccCongAlg_prem0 in Hconcl ; eauto.
+
+  - intros * wu' [Hconcl []]%dup.
+    apply compute_domain.
+    simp _uconv uconv_tm_red build_nf_view2.
+    eapply Uterm_isType in wu' ; tea.
+    destruct wu' ; cbn ; try exact I.
+    now unshelve erewrite whne_nf_view1 ; cbn.
+
+  - intros * w _ ? IH ? w' [Hconcl []]%dup.
+    apply compute_domain.
+    simp _uconv uconv_tm_red build_nf_view2 ; cbn.
+    eapply fun_isFun in w, w' ; eauto.
+    destruct w, w'.
+
+    + eapply LamCongUAlg_prem0 in Hconcl as (?&?&[[=<-<-]]).
+      2: now constructor.
+      cbn ; split ; [..|easy].
+      eapply uconv_expand ; [..|eapply IH ; split] ; eauto.
+      all: try solve [now eapply typing_eta'].
+      2: reflexivity.
+      now eapply redalg_one_step, eta_expand_beta.
+
+    + eapply LamNeUAlg_prem0 in Hconcl as (?&?&[[=<-<-]]).
+      2: now constructor.
+      cbn.
+      unshelve (erewrite whne_nf_view1) ; tea ; cbn.
+      split ; [..|easy].
+      eapply uconv_expand ; [..|eapply IH ; split] ; eauto.
+      all: try solve [now eapply typing_eta'].
+      * eapply redalg_one_step, eta_expand_beta.
+      * reflexivity.
+
+    + eapply NeLamUAlg_prem0 in Hconcl as (?&?&[[=<-<-]]).
+      2: now constructor.
+      cbn.
+      unshelve (erewrite whne_nf_view1) ; tea ; cbn.
+      split ; [..|easy].
+      eapply IH ; split ; eauto.
+
+    + unshelve erewrite whne_nf_view1 ; tea ; cbn.
+      unshelve erewrite whne_nf_view1 ; tea ; cbn.
+      split ; [..|easy].
+      apply uconv_expand_ne_eta ; tea.
+      eapply IH.
+      split.
+      all: now eapply typing_eta'.
+
+  - intros * ?? ?? * wu' [Hconcl []]%dup.
+    apply compute_domain.
+    simp _uconv uconv_tm_red build_nf_view2.
+    eapply Uterm_isType in wu' ; tea.
+    destruct wu' ; cbn ; try exact I.
+    2: now unshelve erewrite whne_nf_view1 ; cbn.
+
+    eapply termSigCongAlg_prem0 in Hconcl as [Hpre0 []]%dup.
+    split ; [eauto | intros [] ; cbn ; [|easy]].
+
+    intros [_ Hpost0]%implem_uconv_graph%uconv_sound_decl ; eauto.
+    eapply termSigCongAlg_prem1 in Hpost0 ; eauto.
+
+  - intros ? t u A'' B'' w _ ? IHf ? IHs * w' [Hconcl []]%dup.
+    apply compute_domain.
+    simp _uconv uconv_tm_red build_nf_view2 ; cbn.
+    eapply sig_isPair in w, w' ; tea.
+    destruct w, w'.
+
+    + cbn.
+      eapply PairCongUAlg_prem0 in Hconcl as (?&?&[[=<-<-] [[]]%dup]).
+      2: now constructor.
+      cbn.
+      split.
+      1:{
+        eapply uconv_expand, IHf ; try reflexivity ; [..|split] ; eauto.
+        2: eapply redalg_one_step ; econstructor.
+        all: now econstructor.
+      }
+
+      intros [] ; cbn ; [|easy].
+      intros [_ Hpost1]%implem_uconv_graph%uconv_sound_decl ; eauto.
+      eapply PairCongUAlg_prem1 in Hpost1 as [] ; eauto.
+      split ; [..|easy].
+      eapply uconv_expand, IHs ; try reflexivity ; [..|split] ; eauto.
+      2: eapply redalg_one_step ; econstructor.
+      all: now econstructor.
+
+    + cbn.
+      eapply PairNeUAlg_prem0 in Hconcl as (?&?&[[=<-<-] [[]]%dup]).
+      2: now constructor.
+      unshelve erewrite whne_nf_view1 ; tea ; cbn.
+      split.
+      1:{
+        eapply uconv_expand, IHf ; try reflexivity ; [..|split] ; eauto.
+        2: eapply redalg_one_step ; econstructor.
+        all: now econstructor.
+      }
+
+      intros [] ; cbn ; [|easy].
+      intros [_ Hpost1]%implem_uconv_graph%uconv_sound_decl ; eauto.
+      eapply PairNeUAlg_prem1 in Hpost1 as [] ; eauto.
+      split ; [..|easy].
+      eapply uconv_expand, IHs ; try reflexivity ; [..|split] ; eauto.
+      2: eapply redalg_one_step ; econstructor.
+      all: now econstructor.
+
+    + cbn.
+      eapply NePairUAlg_prem0 in Hconcl as (?&?&[[=<-<-] [[]]%dup]).
+      2: now constructor.
+      unshelve erewrite whne_nf_view1 ; tea ; cbn.
+      split.
+      1: now eapply uconv_expand, IHf ; try reflexivity ; [..|split].
+
+      intros [] ; cbn ; [|easy].
+      intros [_ Hpost1]%implem_uconv_graph%uconv_sound_decl ; eauto.
+      eapply NePairUAlg_prem1 in Hpost1 as [] ; eauto.
+
+    + cbn.
+      do 2 (unshelve erewrite whne_nf_view1 ; tea ; cbn).
+      split ; [..|easy].
+      eapply uconv_expand_ne_fst ; tea.
+      apply IHf.
+      split ; now econstructor.
+
+  - intros * ?? ?? ?? ? wu' [Hconcl []]%dup.
+    apply compute_domain.
+    simp _uconv uconv_tm_red build_nf_view2.
+    eapply Uterm_isType in wu' ; tea.
+    destruct wu' ; cbn ; try exact I.
+    2: now unshelve erewrite whne_nf_view1 ; cbn.
+
+    eapply termIdCongAlg_prem0 in Hconcl as [Hpre0 []]%dup.
+    split ; [eauto | intros [] ; cbn ; [|easy]].
+
+    intros [_ [Hpost0]%dup]%implem_uconv_graph%uconv_sound_decl ; eauto.
+    eapply termIdCongAlg_prem1 in Hpost0 as [[]]%dup ; eauto.
+    split ; [eauto | intros [] ; cbn ; [|easy]].
+
+    intros [_ Hpost1]%implem_uconv_graph%uconv_sound_decl ; eauto.
+    eapply termIdCongAlg_prem2 in Hpost1 ; eauto.
+
+  - intros * _ * _ * wu' [Hconcl []]%dup.
+    apply compute_domain.
+    simp _uconv uconv_tm_red build_nf_view2.
+    eapply id_isId in wu' ; tea.
+    destruct wu' as [|(?&?&->)] ; cbn ; try exact I.
+    now unshelve erewrite whne_nf_view1 ; cbn.
+
+  - intros * []%algo_conv_wh IH Hpos ? wu' [Hconcl [? Hty]]%dup. 
+    apply compute_domain.
+    simp _uconv uconv_tm_red build_nf_view2.
+    unshelve erewrite whne_nf_view1 ; tea ; cbn.
+    destruct wu' ; cbn ; try easy.
+    + eapply termGen' in Hty as (?&[? [->]]&Hconv).
+      eapply red_ty_compl_prod_l' in Hconv as (?&?&[->]).
+      2: gen_typing.
+      inversion Hpos.
+      inv_whne.
+    + eapply termGen' in Hty as (?&[->]&Hconv).
+      eapply red_ty_compl_sig_l' in Hconv as (?&?&[->]).
+      2: gen_typing.
+      inversion Hpos.
+      inv_whne.
+    + unshelve erewrite whne_nf_view1 ; tea ; cbn.
+      split ; [..|easy].
+      eapply IH ; tea.
+      split ; now eexists.
+ 
+Qed.
